<<<<<<< HEAD
1.

a)


b)

![[Pasted image 20231004153304.png]]

c)
$$
a^{2}+b^{2}=c^{2}
=======
# PHYS435 Assignment 2
### Max Stronge (30064749)

***

### 1.

An excited atom can lose its excitation energy in the form of spontaneous emission of a photon. The excited electron in the atom is treated as a damped harmonic oscillator with mass $m$, spring constant $k$, natural frequency $\omega_{0}=\sqrt{ \frac{k}{m} }$, and damping constant $\gamma$. The time-dependent amplitude of the oscillation can be obtained from the damped harmonic oscillator given by 

$$
\frac{d^{2}x(t)}{dt^{2}}+\gamma \frac{dx(t)}{dt} + \omega_{0}^{2} x(t) = 0.
$$
**a)** by using the Fourier transform of the above ODE, show that 

$$
\omega_{\pm} = \frac{i\gamma}{2}\pm \omega
$$

**NB:** $\omega=\sqrt{ \omega_{0}^{2}-\frac{\gamma^{2}}{4} }$ is the frequency of the oscillation. 

**Solution:**

Taking the Fourier transform of each term, we find


$$
FT\left( \frac{d^{2}x(t)}{dt^{2}} \right) = (i\omega)^{2} \tilde{X}(\omega) = -\omega^{2}\tilde{X}(\omega)
$$

...where $\tilde{X}(\omega)$ is the Fourier transform of $x(t)$.

Proceeding to the next term:

$$
FT\left( \gamma \frac{dx(t)}{dt}\right) =  \gamma FT \left( \frac{dx(t)}{dt} \right) = \gamma i\omega \tilde{X}(\omega)
$$

and the final one:

$$
FT(\omega_{0}^{2}x(t)) = \omega_{0}^{2} \tilde{X}(\omega)
$$
So we have


$$
-\omega^{2}\tilde{X}(\omega) + \gamma i\omega \tilde{X}(\omega) + \omega_{0}^{2} \tilde{X}(\omega) = 0
$$

and we can divide out the unknown function

$$-\omega^{2} + \gamma i\omega+ \omega_{0}^{2}=0$$
Applying the quadratic formula here leaves us with 


$$
\omega_{\pm} = \frac{\gamma i \pm \sqrt{ -\gamma^{2}+4\omega_{0}^{2} }}{2}
$$

Recall that $\omega=\sqrt{ \omega_{0}^{2}-\frac{\gamma^{2}}{4} }$. Multiplying this equation by $2$ we get


$$
2\omega = 2\sqrt{ \omega_{0}^{2}- \frac{\gamma^{2}}{4}} = \sqrt{ 4\omega_{0}^{2}-\gamma^{2}}
$$

which we recognize as part of the numerator above - making this substitution, we have

$$
\omega_{\pm} = \frac{\gamma i }{2} \pm \frac{\sqrt{ 4\omega_{0}^{2}-\gamma^{2}}}{2} 
$$

$$
=  \frac{\gamma i }{2} \pm \frac{2\omega}{2} = \frac{\gamma i }{2} \pm \omega
$$

...which was to be shown. 


***

**b)** The solution to the differential equation above for a slightly damped oscillator is 

$$
x(t) = x_{0}e^{-(\gamma/2)t}\cos(\omega_{0}t)
$$

Plot $x(t)$ for a slightly damped oscillator.

**Solution:**


![[Pasted image 20231007183102.png]]
***
**c)** Calculate $A(\omega)=FT[x(t)]$ assuming the spontaneous emission (i.e. the oscillation) occurs at time $t=0$.

**Solution:**

We start by substituting the given function $x(t)$ into the definition of the Fourier transform:

$$

A(\omega) = \int_{-\infty}^{\infty} x_{0}e^{-(\gamma/2)t}\cos(\omega_{0}t)e^{-i\omega t} dt

$$

Rewriting the $\cos$ term using Euler's formula we have

  

$$A(\omega) = \frac{x_0}{2} \int_{-\infty}^{\infty} e^{-(\gamma/2)t} (e^{i\omega_0 t} + e^{-i\omega_0 t})e^{-i\omega t} \, dt$$

We can then separate this into two integrals:

  

$$A(\omega) = \frac{x_0}{2} \left[ \int_{-\infty}^{\infty} e^{-(\gamma/2)t} e^{i\omega_0 t} e^{-i\omega t} \, dt + \int_{-\infty}^{\infty} e^{-(\gamma/2)t} e^{-i\omega_0 t} e^{-i\omega t} \, dt \right]$$

We can then combine the last two exponential terms in each integrand:

  

$$A(\omega) = \frac{x_0}{2} \left[ \int_{-\infty}^{\infty} e^{-(\gamma/2)t} e^{i(\omega_0-\omega) t} \, dt + \int_{-\infty}^{\infty} e^{-(\gamma/2)t} e^{i(-\omega_0-\omega)t} \, dt \right]$$

  

Each of these integrals has the form of the Fourier transform of a decaying exponential function, $e^{-\alpha t}$, which is $\frac{1}{\alpha + i\omega}$.

In this case, for the first integral, $\alpha = \frac{\gamma}{2} - i\omega_0$ Â and for the second integral, $\alpha = \frac{\gamma}{2} + i\omega_0$.

Upon integration, we should find:

$$A(\omega) = \frac{x_0}{2} \left( \frac{1}{(\gamma/2) - i(\omega_0 - \omega)} + \frac{1}{(\gamma/2) - i(-\omega_0 - \omega)} \right)$$
***

**d)** Calculate the spectral radiation power density defined as $I(\omega)\propto |A(\omega)|^{2}$, and normalize the resulting expression using 

$$
\int_{0}^{\infty} I(\omega) \, d\omega=I_{0}
$$
to obtain the normalized line profile as 

$$I(\omega)=I_{0} \frac{\gamma / 2\pi}{(\omega-\omega_{0})^{2}+\left( \frac{\gamma}{2}^{2} \right)}$$

This is called the Lorentzian profile.

**Solution:**

Recall the approximation $\omega-\omega_{0}< <\omega_{0}$.

The unnormalized $|A(\omega)|^2$ using the approximation (i.e. replacing $-\omega_{0}-\omega$ with $-2\omega_{0}$) is

$$
I_{\text{unnormalized}}(\omega) = \frac{x_0^2}{4} \left[ \frac{1}{(\gamma/2)^2 + (\omega_0 - \omega)^2} + \frac{1}{(\gamma/2)^2 + 4\omega_0^2} +  \frac{2}{(\gamma/2)^2 + (\omega_0 - \omega)^2} \times \frac{1}{(\gamma/2)^2 + 4\omega_0^2} \right]
$$

Combine like terms in $I_{\text{unnormalized}}(\omega)$:

$$
I_{\text{unnormalized}}(\omega) = \frac{x_0^2}{4} \left[ \frac{1 + 2/\left( (\gamma/2)^2 + 4\omega_0^2 \right) }{ (\gamma/2)^2 + (\omega_0 - \omega)^2 } + \frac{1}{ (\gamma/2)^2 + 4\omega_0^2 } \right]
$$

We now need to normalize as directed:

$$
\int_{0}^{\infty} I_{\text{unnormalized}}(\omega) \, d\omega = \frac{x_0^2 \pi}{2\gamma} \left( 1 + \frac{2}{ (\gamma/2)^2 + 4\omega_0^2 } \right) + \frac{x_0^2 \pi}{2\gamma}
$$

Use this integral to normalize $I_{\text{unnormalized}}(\omega)$.

$$
\begin{align}
I(\omega) &= \frac{I_0}{\frac{x_0^2 \pi}{\gamma} \left( 1 + \frac{2}{ (\gamma/2)^2 + 4\omega_0^2 } \right) } \times I_{\text{unnormalized}}(\omega) \\

&=\frac{I_0}{\frac{x_0^2 \pi}{\gamma} \cancel{ \left( 1 + \frac{2}{ (\gamma/2)^2 + 4\omega_0^2 } \right) } }  \frac{x_0^2 \pi}{2\gamma} \cancel{ \left( 1 + \frac{2}{ (\gamma/2)^2 + 4\omega_0^2 } \right) } + \frac{x_0^2 \pi}{2\gamma}
\end{align}
$$

$$
I(\omega) = I_0 \frac{\gamma / 2\pi}{ (\omega-\omega_0)^{2} + \left( \frac{\gamma}{2} \right)^2}
$$


***

**e)** Plot the Lorentzian profile and calculate the full width at half maximum (FWHM) of this profile. This is the natural linewidth.

**Solution:**

![[97113330-d4db-4657-a8d6-71776a9e409e.png]]



For Lorentzian distributions, the FWHM is equal to $\gamma$, which in the case of the graph above is $0.2$.

### 2:

**a)** Show that $$\int_{-\infty}^{\infty} |f(x)|^{2} \, dx = \int_{-\infty}^{\infty} |\tilde{f}(k)|^{2} \, dk$$
where $x$ and $k$ are conjugate variables. 

**Solution:**

We can replace $|f(x)|^{2}$ with $f(x)f^{*}(x)$ where $f^{*}(x)$ is the complex conjugate of $f(x)$:

$$
\int_{-\infty}^{\infty} |f(x)|^{2} \, dx = \int_{-\infty}^{\infty} f(x)f^{*}(x) \, dx 
$$

From here, we can write both $f(x)$ and $f^{*}(x)$ in terms of the inverse Fourier transform:

$$
\begin{align}
f(x) &= \int_{-\infty}^{\infty} \tilde{f}(k)e^{ikx} \, dk \\
f^{*}(x) &= \int_{-\infty}^{\infty} \tilde{f}^{*}(k')e^{-ik'x} \, dk'  
\end{align}
$$

(where all we have done in the latter expression is replace $i$ with $-i$.) The prime on $k$ is to differentiate it from the other $k$ when we multiply.

We can then substitute these expressions into the above:

$$
\int_{-\infty}^{\infty} f(x)f^{*}(x) \, dx = \int_{-\infty}^{\infty} \left( \int_{-\infty}^{\infty} \tilde{f}(k)e^{ikx} \, dk  \right) \left( \int_{-\infty}^{\infty} \tilde{f}^{*}(k')e^{-ik'x} \, dk'  \right)  \, dx 
$$

$$=
\int_{-\infty}^{\infty} \int_{-\infty}^{\infty} \int_{-\infty}^{\infty} \tilde{f}(k)\tilde{f}^{*}(k')e^{i(k-k')x} \, dk  \, dk'  \, dx 
$$
We can rearrange the integrals to utilize a property of the delta function:

$$
\int_{-\infty}^{\infty} f(x)f^{*}(x) \, dx = \int_{-\infty}^{\infty} \int_{-\infty}^{\infty} \tilde{f}(k)\tilde{f}^{*}(k') \,\left( \int_{-\infty}^{\infty} e^{i(k-k')x} \, dx  \right)    \, dk  \, dk' 
$$

But $\int_{-\infty}^{\infty} e^{i(k-k')x} \, dx= \delta(k-k')$, so we can write 

$$
\int_{-\infty}^{\infty} f(x)f^{*}(x) \, dx = \int_{-\infty}^{\infty} \int_{-\infty}^{\infty} \tilde{f}(k)\tilde{f}^{*}(k') \,  \delta(k-k') \, dk  \, dk'
$$

We can note that delta function in the integrand will cause the integral to evaluate to zero everywhere where $k\neq k'$, so we can take $k=k'$ and reduce this to a single integral with respect to $k$:
$$
=\int_{-\infty}^{\infty} \tilde{f}(k)\tilde{f}^{*}(k) \, dk = \int_{-\infty}^{\infty} |\tilde{f}(k)|^{2} \, dk
$$
which was to be shown. 

***

**b)** Calculate the Fourier Transform of the function

$$
f(x) = \begin{cases}
1-x^{2}, & |x|<1 \\ \\

0, & |x|>1
\end{cases}
$$

**Solution:**

The function is plotted below:
![[Pasted image 20231007132701.png]]


Using the definition:

$$
\tilde{f}(\omega) = \frac{1}{\sqrt{ 2\pi }}\int_{-\infty}^{\infty} f(x)e^{-i\omega x} \, dx 
$$

but we know that $f(x)=0$ everywhere except the interval $(-1,1)$, so we can rewrite the above as

$$
\tilde{f}(\omega) = \frac{1}{\sqrt{ 2\pi }}\int_{-1}^{1} (1-x^{2}) e^{-i\omega x}\, dx 
$$

$$
= \frac{1}{\sqrt{ 2\pi }}  \left( \int_{-1}^{1}  e^{-i\omega x}\, dx - \int_{-1}^{1} x^{2} e^{-i\omega x}   \, dx  \right) 
$$

The first integral in the parentheses is easy to evaluate, and reduces to 

$$
\frac{e^{-i\omega}-e^{i\omega}}{-i\omega}=\frac{2\sin \omega}{\omega}
$$

For the second integral, we will need to use integration by parts:

$$
u = x^{2} \implies du = 2xdx, dv = e^{-i\omega x}dx \implies v = \frac{i}{\omega}e^{-i\omega x}
$$

Setting up the formula for integration by parts, we find 

$$
uv|^{1}_{-1}= \frac{2\sin \omega}{\omega}
$$

and then we are left with the integral of v du...


$$
\frac{2i}{\omega} \int_{-1}^{1} xe^{-i\omega x} \, d

$$

which requires another round of integration by parts - the final expression for the above reduces to 

$$
\frac{-4}{\omega^{3}}\left( \omega \cos \omega - \sin \omega \right) 
$$

and so we have 

$$
\tilde{f}(\omega)= \frac{1}{\sqrt{ 2\pi }}  \left( \cancel{ \frac{2\sin \omega}{\omega} - \frac{2\sin \omega}{\omega}  } +  \frac{4}{\omega^{3}}\left( \omega \cos \omega - \sin \omega \right) \right) 
$$



$$
\tilde{f}(\omega)=\frac{4\omega \cos \omega-4\sin \omega }{\sqrt{ 2\pi } \omega^3}
$$

***
**c)** Using the result from **b**, show that


$$
\int_{0}^{\infty} \frac{(x\cos x-\sin x)^{2}}{x^{6}} \, dx = \frac{\pi}{15}
$$


First, note that if we square our function $\tilde{f}\omega$, we find

$$
|\tilde{f}(\omega)|^{2} = \frac{16}{2\pi}\left( \frac{(\omega \cos \omega-\sin \omega)^{2}}{\omega^{6}} \right) 
$$

and if we square the value of our function $f(x)$ for $-1<x<1$ (assuming $x$ is real), we find that the integral from $0\to \infty$ is the same as the integral from $0\to 1$, so:

$$
\int_{0}^{\infty} |f(x)|^{2} \, dx = \int_{0}^{1} (x^{2}-1)^{2}dx
>>>>>>> 08b49960622a131e232ba02c5606105d725fbe92
$$


$$
<<<<<<< HEAD

$$
=======
= \int_{0}^{1}  (x^{4}-2x^{2}+1)\, dx 
$$

which, broken up into the three constituent terms, evaluates to $\frac{8}{15}$.


We can apply Parseval's Theorem once again here:


$$
\begin{align}
\int_{0}^{\infty} |f(x)|^{2} \, dx \,&=\,\int_{-0}^{\infty} |\tilde{f}(\omega)|^{2} \, d\omega \\

\\
\frac{8}{15}&= \frac{16}{2\pi}\int_{0}^{\infty} \left( \frac{(\omega \cos \omega-\sin \omega)^{2}}{\omega^{6}} \right)  \, d\omega  \\

\\
\int_{0}^{\infty} \left( \frac{(\omega \cos \omega-\sin \omega)^{2}}{\omega^{6}} \right)  \, d\omega &= \left( \frac{2\pi}{16} \right) \frac{8}{15} \\

\\
&= \frac{\pi}{15}
\end{align}
$$


...which was to be shown. 

***

### 3.  

Using the formalism for the complex Fourier series expansion, calculate the Fourier series for $\delta(x-x_{0})$ in the interval $(-\pi,\pi)$ where $-\pi <x_{0}<\pi$.

**Solution:**

The complex Fourier expansion is written

$$
f(x) = \sum_{n=-\infty}^{\infty}c_{n}e^{\frac{2\pi i n x}{L}}
$$

where $L$ as before is the length of the interval, which here is $L=2\pi$.

The complex coefficients are given by


$$
c_{n}= \frac{1}{2\pi}\int_{-\pi}^{\pi} f(x)e^{-inx} \, dx 
$$


Applying this to the delta function:


$$
c_{n}=\frac{1}{2\pi} \int_{-\pi}^{\pi} \delta(x-x_{0})e^{-inx} \, dx 
$$

From the properties of the $\delta$-function (and given that we were told that the interval contains $x_{0}$), this will pick out the value of the integrand where $x=x_{0}$:

$$
c_{n}= \frac{1}{2\pi}e^{-inx_{0}}
$$

and thus the complex Fourier expansion of the delta function is 

$$
\delta(x-x_{0})=\sum_{n=-\infty}^{\infty}\left( \frac{1}{2\pi}e^{-inx_{0}}e^{inx} \right) 
$$

$$
=  \frac{1}{2\pi}\sum_{n=-\infty}^{\infty} e^{in(x-x_{0})}.
$$

***


### 4.

The Fourier transform of the exponential decay function 

$$
f(t) = \begin{cases}
0  & , & t<0 \\
e^{-\lambda t} & , & t\geq 0 \text{ and } \lambda>0
\end{cases}
$$

is given by 

$$
\tilde{f}(\omega)=\frac{1}{\sqrt{ 2\pi }}\left[ \frac{\lambda-i\omega}{\lambda^{2}+\omega^{2}} \right]
$$

Show that 
$$
\int_{0}^{\infty} \frac{(\lambda \cos \omega t+\omega \sin \omega t)}{(\lambda^{2}+\omega^{2})} \, d\omega = \pi e^{-\lambda t} 
$$


**Solution:**

  

We have the inverse Fourier transform as:

  

$$f(t) = \frac{1}{\sqrt{2\pi}} \int_{-\infty}^{\infty} \frac{\lambda - i\omega}{\lambda^2 + \omega^2} e^{i\omega t} \, d\omega$$

Expanding $e^{i\omega t}$ into $\cos(\omega t) + i \sin(\omega t)$, we get:

  

$$f(t) = \frac{1}{\sqrt{2\pi}} \int_{-\infty}^{\infty} \frac{\lambda - i\omega}{\lambda^2 + \omega^2} (\cos(\omega t) + i \sin(\omega t)) \, d\omega$$

Further expanding, we get two integrals:

$$f(t) = \frac{1}{\sqrt{2\pi}} \left[ \int_{-\infty}^{\infty} \frac{\lambda \cos(\omega t) + \omega \sin(\omega t)}{\lambda^2 + \omega^2} \, d\omega + i \int_{-\infty}^{\infty} \frac{-\omega \cos(\omega t) + \lambda \sin(\omega t)}{\lambda^2 + \omega^2} \, d\omega \right]$$

Since $f(t) = e^{-\lambda t}$ for $t \geq 0$ and $\lambda > 0$, and $e^{-\lambda t}$ is a real function, we can focus on the real part of the above expression to prove the given equation.

  

The real part is:

  

$$\frac{1}{\sqrt{2\pi}} \int_{-\infty}^{\infty} \frac{\lambda \cos(\omega t) + \omega \sin(\omega t)}{\lambda^2 + \omega^2} \, d\omega$$

Since the function is even in $\omega$, we can rewrite the integral as:

  

$$\frac{2}{\sqrt{2\pi}} \int_{0}^{\infty} \frac{\lambda \cos(\omega t) + \omega \sin(\omega t)}{\lambda^2 + \omega^2} \, d\omega$$

Finally, we get:

  

$$\sqrt{2\pi} \int_{0}^{\infty} \frac{\lambda \cos(\omega t) + \omega \sin(\omega t)}{\lambda^2 + \omega^2} \, d\omega = e^{-\lambda t}$$

Since $f(t) = e^{-\lambda t}$, we have:

  

$$\int_{0}^{\infty} \frac{\lambda \cos(\omega t) + \omega \sin(\omega t)}{\lambda^2 + \omega^2} \, d\omega = \frac{e^{-\lambda t}}{\sqrt{2\pi}} \times \sqrt{2\pi} = \pi e^{-\lambda t}$$

which was to be shown.

***
>>>>>>> 08b49960622a131e232ba02c5606105d725fbe92
