# 3.4 - The Compton Effect:
***

Another way for radiation to interact with matter is by means of the **Compton effect**, in which radiation scatters from loosely bound, nearly free electrons. Part of the energy of the radiation is given to the electron; the remainder of the energy is reradiated as electromagnetic radiation. According to our theory of waves, the scattered radiation is less energetic than the **incident radiation** (with the difference going into the kinetic energy of the electron), but *has the same wavelength*. The photon concept, however, leads to a very different prediction for the scattered radiation.

The scattering process is analyzed simply as a **collision** between a single photon and an electron, which we assume to be at rest. 

![[Pasted image 20210421142328.png]]

Initially, the photon has energy $E$ and linear momentum $p$ given by:

> ## $$E = hf= \frac{hc}{\lambda}\quad \text{and}\quad p - \frac{E}{c} .$$

The electron, initially at rest, has rest energy $m_ec^2$ (this is the total energy of the electron at this point). After scattering, the photon has energy $E' = hc/\lambda'$ and momentum $p' = E'/c$, and it will scatter off in a direction of angle $\theta$ with respect to the initial direction of the photon. The electron has total final energy $E_e$ and momentum $p_e$ and moves off at an angle $\phi$ (with respect to the initial direction of the photon as well).

We then can apply the [[2.7 - Relativistic Dynamics#^51a1a3|conservation laws for relativistic dynamics]]:

>  $$\LARGE
> \begin{align}
E_{initial} = E_{final}&: \qquad E + m_ec^2 = E' + E_e\\
p_{x,initial} = p_{x,final}&: \qquad p = p_e\cos(\phi)+p'\cos(\theta)\\
p_{y,initial} = p_{y,final}&:\qquad 0 = p_e\sin(\phi) - p'\sin(\theta).
> \end{align} $$

Here we have three equations with four unknowns that cannot be solved uniquely, but we can eliminate any four of the two unknowns by solving the equations *simultaneously*.

After some algebra, we can find the following expressions eliminating the energy and direction of the scattered photon:

> ## $$\frac{1}{E'}-\frac{1}{E} = \frac{1}{m_ec^2}\left(1-\cos(\theta)\right). $$

We can also put this in terms of the wavelength: 

> ## $$\lambda' - \lambda = \Delta \lambda = \frac{h}{m_ec}(1-\cos(\theta)) $$
> ....where $\lambda$ is the wavelength of the **incident** photon and $\lambda'$ is the wavelength of the **scattered** photon. 