# Proof Assignment Week 1:

***


Suppose $\bf{A}$ and $\bf{B}$ are two skew-symmetric matrices (*i.e.* $\bf{A}^T = -\bf{A}, \bf{B}^T = -\bf{B}$). Suppose $\bf{AB} = \bf{BA}$ (the two matrices are commutative). 

First, let's analyze the first statement: the matrix $\bf{AB}$, as defined above, is *skew-symmetric*.

If $\bf{AB}$ is skew-symmetric, then by definition, $\bf{AB}^T = -(\bf{AB})$. The left hand side, by the properties of the transpose of matrix products, is equivalent to $\bf{B}^T\bf{A}^T$, so that:


