# PHYS435 Assigment 6
### Max Stronge (30064749)

***


1. Show that 
$$
P_{n}(z)=\frac{1}{2\pi i} \oint \frac{(t^{2}-1)^{n}}{2^{n}(t-z)^{n+1}}dt

$$

**Solution:**

Starting from Rodrigues' formula for Legendre polynomials, we have

$$
P_{n}(z) = \frac{1}{2^{n}n!} \frac{d^{n}}{dz^{n}}\left[ (z^{2}-1)^{n} \right] 
$$

Cauchy's integral formula gives us a way to relate the $n$-th derivative to an integral over a contour in the complex plane:

$$
f^{(n)}(z_{0}) = \frac{n!}{2\pi i}\oint \frac{f(z)dz}{(z-z_{0})^{n+1}}
$$
or, replacing $z$ with $t$ and $z_{0}$ with $z$, and rewriting the $n$-th derivative to look more like the form in Rodrigues' formula:

$$
\frac{d^{(n)}}{dz^{n}}f(z) = \frac{n!}{2\pi i} \oint \frac{f(t)}{(t-z)^{n+1}}dt
$$

This is valid if $f(t)$ is analytic within the closed contour. Legendre's equation has regular singularities at $z=\pm 1$ (as well as $\infty$), and is analytic at $z=0$, so our contour is the circle of $|z|<1$.

In Rodrigues' formula, $f(z)=(z^{2}-1)^{n}$ or, with our change of variables, $f(t)(t^{2}-1)^{n}$, so we can say using Cauchy's formula

$$
\frac{d^{n}}{dz^{n}}(z^{2}-1)^{n} = \frac{n!}{2\pi i}\oint \frac{(t^{2}-1)^{n}}{(t-z)^{n+1}}dt
$$

If we put substitute this back into Rodrigues' formula we find

$$
\begin{align}
P_{n}(z) &= \frac{1}{2^{n}\cancel{ n! }} \frac{\cancel{ n! }}{2\pi i}\oint \frac{(t^{2}-1)^{n}}{(t-z)^{n+1}}dt  \\ \\

&= \frac{1}{2\pi i} \frac{1}{2^{n}} \oint \frac{(t^{2}-1)^{n}}{(t-z)^{n+1}}dt  \\ \\

&= \frac{1}{2\pi i}\oint \frac{(t^{2}-1)^{n}}{2^{n}(t-z)^{n+1}}dt 

\end{align}


$$

which was to be shown.


***



2. 

**a)** Show that $\int_{-1}^{1} P_{n}(x) P_{n}(x) \, dx=\frac{2}{2n+1}$ using the generating function for $P_{n}(x)$. 


**Solution:**

The generating function for the Legendre polynomials $P_{n}(x)$ is given by

$$
G(x,h) = (1-2xh+h^{2})^{-1/2} = \sum_{n=0}^\infty P_{n}(x)h^{n}
$$
We want to to show that the integral of the product of $P_{n}(x)$ with itself is equal to some function of $n$, so let's square both sides of the above:

$$
\frac{1}{1-2xh+h^{2}}= \sum_{n=0}^\infty \sum_{m=0}^\infty P_{n}(x)P_{m}(x)h^{n+m}
$$
where the double series is introduced because to square the sum of $P_{n}$, each term of it must be multiplied by each other term (including both the cases where $m=n$ and $m\neq n$). We can then integrate both sides with respect to $x$ from $-1$ to $1$:

$$
\begin{align}
\int_{-1}^{1} \frac{1}{1-2xh+h^{2}} \, dx &= \int_{-1}^{1} \sum_{n=0}^\infty \sum_{m=0}^\infty P_{n}(x)P_{m}(x)h^{n+m} \, dx  \\
\\
-\frac{1}{2h}\ln(1-2xh+h^{2})\biggr\rvert^1_{-1} &= \sum_{n=0}^\infty \sum_{m=0}^\infty\int_{-1}^{1} P_{n}(x)P_{m}(x) h^{n+m}\, dx
\end{align}
$$

...where in the second step the order of the integral and the sums has been reversed. At this stage we can employ the orthogonality property of the Legendre polynomials to note that the integral on the right hand side will be equal to zero everywhere $n\neq m$, so we will be left only with the terms where $n=m$. Evaluating the expression on the left hand side at the limits and simplifying, we find

$$
\frac{1}{h}\ln \left( \frac{h+1}{h-1} \right)  = \sum_{n=0}^\infty \sum_{m=0}^\infty I_{n} \delta_{nm}h^{n+m}
$$
where $I_{n}$ is the value of the integral we are trying to find, $\int_{-1}^{1} P_{n}(x)^{2} \, dx$, and the Kroenecker delta shows that the integral in the previous step is equal to $I_{n}$ when $m=n$ and $0$ otherwise. In this case, since $m=n$, we can replace $h^{n+m}$ with $h^{2n}$ and revert to a single series over $n$, as the other is unnecessary:

$$
\sum_{n=0}^\infty I_{n} h^{2n} = \frac{1}{h}\ln \left( \frac{h+1}{h-1} \right)
$$

To manipulate the right hand side of this equation such that we can identify the value of $I_{n}=\int_{-1}^{1} P_{n}(x) \, dx$, we need to put it into a form that is also a power series - then, equating like powers of $h$ to give the values of $I_{n}$. We can use the Taylor series expansion of $\ln(h+1)$ and $\ln(h-1)$:

$$
\ln \left( \frac{h+1}{h-1} \right) = \ln(h+1)-\ln(h-1) = \left( \sum_{n=0}^\infty \frac{(-1)^{n}h^{n+1}}{n+1} - \sum_{n=0}^\infty \frac{(-1)h^{n+1}}{n+1} \right) 
$$

$$
= \frac{2h^{n}}{n+1} \text{for even }n\text{, or } \frac{2h^{2n}}{2n+1}.
$$

Thus we have 
$$
 I_{n} \cancel{ h^{2n} } = \frac{2\cancel{ h^{2n} }}{2n+1}
$$

$$
I_{n} = \int_{-1}^{1} P_{n}(x)P_{n}(x) \, dx = \frac{2}{2n+1}. 
$$



**b)** Show that $\int_{-\infty}^{\infty} H_{m}(x) H_{n}(x)e^{-x^{2}} \, dx=2^{n}n!\sqrt{ \pi }\delta_{mn}$.

**Solution:** The generating function of the Hermite polynomials is 

$$
G(x,h) = e^{-h^{2}+2hx}=\sum_{n=0}^\infty \frac{H_{n}(x)}{n!}h^{n}
$$
Following a similar procedure as the previous question, we square both sides:

$$
e^{-2h^{2}-4hx}=\sum_{n=0}^\infty\sum_{m=0}^\infty \frac{H_{n}(x)H_{m}(x)}{n!m!}h^{n+m}
$$

And again we integrate both sides, this time adding the weight function $e^{-x^{2}}$:

$$
\int_{-\infty}^{\infty} e^{-2h^{2}-4hx-x^{2}} \, dx = \int_{-\infty}^{\infty} \sum_{n=0}^\infty\sum_{m=0}^\infty \frac{H_{n}(x)H_{m}(x)}{n!m!}h^{n+m} e^{-x^{2}}\, dx  
$$

Again we invoke the fact that the Hermite polynomials are orthogonal, and this RHS will be equal to zero for all $m\neq n$. This takes care of the $\delta_{mn}$ part, so what we now need to show is 

$$
\int_{-\infty}^{\infty} H_{n}(x) H_{n}(x)e^{-x^{2}} \, dx=2^{n}n!\sqrt{ \pi }
$$

We can again switch the order of integration/summation:

$$
\int_{-\infty}^{\infty} e^{-2h^{2}-4hx-x^{2}} \, dx = \sum_{n=0}^\infty\int_{-\infty}^{\infty}  \frac{H_{n}(x)^{2}}{(n!)^{2}}h^{2n} e^{-x^{2}}\, dx  
$$
To evaluate the integral on the left-hand side, we can factor it by completing the square:

$$
e^{-2h^{2}-4hx-x^{2}} = e^{-(x^{2}+4hx +4h^{2})+2h^{2}} = e^{-(x+2h)^{2}}e^{2h^{2}}
$$
and since the second exponential term is constant in $x$, we can factor it out of the integral, which becomes a Gaussian integral:


$$
\int_{-\infty}^{\infty} e^{-2h^{2}-4hx-x^{2}} \, dx =e^{2h^{2}} \int_{-\infty}^{\infty} e^{-(x+2h)^{2}} \, dx = e^{2h^{2}} \sqrt{ \pi }
$$
If we re-equate this to the RHS of the series of the integral of the square of the Hermite polynomials we have

$$
\sqrt{ \pi }e^{2h^{2}}= \sum_{n=0}^\infty\int_{-\infty}^{\infty}  \frac{H_{n}(x)^{2}}{(n!)^{2}}h^{2n} e^{-x^{2}}\, dx  
$$
As before we need a series representation of the term containing $h$ on the left hand side so we can equate the appropriate coefficients. The series representation of $e^{2h^{2}}$ is given by

$$
e^{2h^{2}}=\sum_{n=0}^\infty \frac{2^{n}(h^{2})^{n}}{n!} = \sum_{n=0}^\infty \frac{2^{n}h^{2n}}{n!}
$$

And so 
$$
\sqrt{ \pi }\sum_{n=0}^\infty \frac{2^{n}h^{2n}}{n!} = \sum_{n=0}^\infty\int_{-\infty}^{\infty}  \frac{H_{n}(x)^{2}}{(n!)^{2}}h^{2n} e^{-x^{2}}\, dx  
$$
Equating the coefficients in the two series:

$$
\begin{align}
\sqrt{ \pi } \frac{2^{n}\cancel{ h^{2n} }}{n!} &= \int_{-\infty}^{\infty}  \frac{H_{n}(x)^{2}}{(n!)^{2}}\cancel{ h^{2n} } e^{-x^{2}}\, dx  \\
  \\
\sqrt{ \pi } \frac{2^{n}}{n!} &= \frac{1}{(n!)^{2}}\int_{-\infty}^{\infty}  H_{n}(x)^{2}e^{-x^{2}}\, dx  \\
  \\
2^{n}n!\sqrt{ \pi }&=\int_{-\infty}^{\infty}  H_{n}(x)^{2}e^{-x^{2}}\, dx 
\end{align}
$$

And as mentioned above, because of the orthogonality of the Hermite polynomials, we can replace $H_{n}(x)^{2}$ with $H_{n}(x)H_{m(x)}$ so long as we introduce the Kroenecker delta:

$$
\int_{-\infty}^{\infty} H_{n}(x)H_{m}(x)e^{-x^{2}} \, dx  = 2^{n}n!\sqrt{ \pi }\delta_{mn}
$$

***


3. Show that 

$$
\int_{-1}^{1} x^{m}P_{n}(x) \, dx = \begin{cases}
0 & n>m \\ \\
\frac{2^{n+1}\left[ (n)! \right] ^{2}}{(2n+1)!} & n=m
\end{cases}
$$
Hint: use

$$
\int_{-1}^{1} (1-x^{2})^{n} \, d = \frac{2^{2n+1}(n!)^{2}}{(2n+1)!}
$$
**Solution:**

Starting from the LHS, we can replace $P_{n}(x)$ with its definition according to Rodrigues' formula:

$$
\int_{-1}^{1} x^{m}P_{n(x)} \, dx=\int_{-1}^{1} x^{m} \left( \frac{1}{2^{n}n!} \frac{d^{n}}{dx^{n}} (x^{2}-1)^{n} \right)  \, dx  
$$

$$
= \frac{1}{2^{n}n!}\int_{-1}^{1} x^{m}\frac{d^{n}}{dx^{n}} (x^{2}-1)^{n} \, dx 
$$

The form of the integrand looks consists of the product of an algebraic part and a differential part, which leads one to think that integration by parts may be in order. Taking $u=x^{m}$ and $dv= \frac{d^{n}}{dx^{n}}(x^{2}-1)^{n}dx$, we have

$$
du = mx^{m-1}dx
$$
and 
$$
v = \int  = \frac{d^{n}}{dx^{n}}(x^{2}-1)^{n}\, dx  =  \frac{d^{n-1}}{dx^{n-1}}(x^{2}-1)^{n}
$$
and so the integral above can be rewritten as 

$$
\frac{1}{2^{n}n!} \left( x^{m} \frac{d^{n-1}}{dx^{n-1}}(x^{2}-1)^{n} \biggr\vert^{1}_{-1} - \int_{-1}^{1} \frac{d^{n-1}}{dx^{n-1}}(x^{2}-1)^{n} mx^{m-1} \, dx \right) 
$$
The left term in the parentheses will be zero at $x=\pm1$, so this reduces to 

$$
\frac{1}{2^{n}n!} \left( - \int_{-1}^{1} \frac{d^{n-1}}{dx^{n-1}}(x^{2}-1)^{n} mx^{m-1} \, dx \right) 
$$
or 

$$
-\frac{m}{2^{n}n!} \int_{-1}^{1} \frac{d^{n-1}}{dx^{n-1}}(x^{2}-1)^{n} x^{m-1}  \, dx 
$$

We need to show that this expression reduces to zero when $n>m$ and to $\frac{2^{n+1}\left[ (n)! \right] ^{2}}{(2n+1)!}$ for $n=m$. 


***

4. 

**a)** Consider the electrostatic potential produced by a thin conducting ring of radius $a$ placed symmetrically in the equatorial plane of a spherical polar coordinate system and carrying a total electric charge $q$ as shown in the figure below. 

![[Pasted image 20231207185026.png]]

Given that the potential $V(\vec{r})$ satisfies Laplace's equation, obtain an expression for $V(r,\theta)$ when $r>a$. Note that $V(\vec{r})$ must go to zero as $r \to \infty$. 

**b)** Show that the expression obtained for a general point in **a)** reduces to 

$$
V(z,\theta=0) = \frac{q}{4\pi \epsilon_{0}(z^{2}+a^{2})^{1/2}}
$$

for points on the $z$ axis. 


**Solution:** As advised in the follow-up email, we tackle these problems in reverse order. First, for $\theta=0$ (i.e. points on the $z$-axis), we can arrive at a simple model for the potential using the expression for the potential due to a point charge:

$$
V(r)= \frac{1}{4\pi \epsilon_{0}} \frac{q}{r}
$$
...where $r$ is the distance away from the point charge giving rise to the potential. On the $z$-axis, the distance away from each infinitesimal part of the ring is $\sqrt{ z^{2}+a^{2} }$, and the fact that we have azimuthal symmetry and are holding $\theta=0$ leaves us with a simple expression for the potential

$$
V(r=z,\theta=0)=\frac{1}{4\pi \epsilon_{0}} \int \frac{1}{\sqrt{ z^{2}+a^{2} }}\,dq  = \frac{q}{4\pi \epsilon_{0}\sqrt{ z^{2}+a^{2} }}. 
$$

The symmetry of this problem simplified the derivation of this expression considerably. 

We now want to obtain an expression that is valid for any $r>a$ and any $\theta$. 

We are told that the potential satisfies Laplace's equation, which in polar spherical coordinates is

$$
\nabla^{2}V = \frac{1}{r^{2}} \frac{ \partial }{ \partial r } \left( r^{2} \frac{ \partial V }{ \partial r } \right) + \frac{1}{r^{2}\sin \theta}\frac{ \partial  }{ \partial \theta } \left( \sin \theta \frac{ \partial V }{ \partial \theta }  \right) =0 
$$

Since we still have azimuthal symmetry, there will be no dependence on $\phi$. We are looking for 

$$
V(r,\theta)
$$
and, using separation of variables, we search for a solution in the form of a product of functions of each of the input variables, i.e. 

$$
V(r,\theta) = R(r)\Theta (\theta)
$$

If we substitute this into Laplace's equation we can take advantage of the fact that each function is dependent on only one variable to turn the partial derivates into full derivatives:

$$
\frac{1}{R} \frac{d}{dr}\left( r^{2} \frac{dR}{dr} \right) + \frac{1}{\Theta \sin \theta} \frac{d}{d\theta} \left( \sin \theta\frac{ d\Theta}{d\theta} \right) =0
$$
..where we have multiplied by $r^{2}$ and divided by $V$ to simplify the equation.

Since the first term is dependent only on $r$ and the second is dependent only on $\theta$, each of these must be a constant which is traditionally in the form $\pm l(l+1)$:

$$
\frac{d}{dr}\left( r^{2} \frac{dR}{dr} \right) = l(l+1)R
$$
and 

$$
\frac{d}{d\theta} \left( \sin \theta  \frac{d\Theta}{d\theta} \right)=-l(l+1)\sin \theta \,\Theta 
$$

The radial equation $R(r)$ has the general solution 

$$
R(r) = Ar^{l} + \frac{B}{r^{l+1}}
$$

and the solutions to the angular equation are Legendre polynomials of $\cos \theta$:

$$
\Theta(\theta) = P_{l}(\cos \theta)$$
and so the most general separable solution is 

$$
V(r,\theta) = \left( Ar^{l} + \frac{B}{r^{l+1}} \right) P_{l}(\cos \theta)
$$

but since the separation of variables produces an infinite number of solutions, the most general is a linear combination of them

$$
V(r,\theta) = \sum_{l=0}^\infty \left( A_{l}r^{l} + \frac{B_{l}}{r^{l+1}} \right) P_{l}(\cos \theta)
$$

Our given boundary conditions allow us to simplify this further - we want the potential to vanish as $r\to \infty$, so we take all $A_{l}$ to be zero, $V$ would be infinite at an infinite distance. Since we are strictly looking for solutions in the region $r>a$, we do not need to worry about the potential exploding to infinity at the origin due to the $B_{l}$ term. 


$$
V(r,\theta) = \sum_{l=0}^\infty \left(\frac{B_{l}}{r^{l+1}} \right) P_{l}(\cos \theta)
$$
The other 'boundary condition' we require is that this expression reduce to the previous one:

$$
V(r=z,\theta=0)=\frac{q}{4\pi \epsilon_{0}\sqrt{ z^{2}+a^{2} }}
$$
...for points on the $z$-axis. Luckily for $\theta=0$, $\cos \theta=1$ and $P_{l} (1) = 1$ for all $l$, so this simplifies our potential to 

$$
V(r,\theta=0) = \sum_{l=0}^\infty \left(\frac{B_{l}}{r^{l+1}} \right)
$$
and our task is to find the coefficients $B_{l}$ that will allow our expression to reduce to the correct simplified one for $\vec{r}=r \hat{z}$. We can replace $r$ with $\sqrt{ z^{2}+a^{2} }$ for points on the $z$-axis:

$$
V(r=z,\theta=0) = \sum_{l=0}^\infty \left(\frac{B_{l}}{(\sqrt{ z^{2}+a^{2} })^{l+1}} \right)
$$
Since $\sqrt{ z^{2}+a^{2} }$ appears with a multiplicity of only 1 in the denominator of the simplified expression, we can neglect all terms in the series except $B_{0}$ which will give the correct form for the denominator. 

$$
V(r=z,\theta=0) =  \frac{B_{0}}{(\sqrt{ z^{2}+a^{2} })}
$$
From this, we can immediately see that the coefficient $B_{0}$ has the value

$$
B_{0}=\frac{q}{4\pi \epsilon_{0}}
$$
and the general solution reduces to the simplified case. 



NB: Derivation of the potential followed Griffith's method in Electrodynamics, Chapter 3.3 Separation of Variables.
***

5. A neutral conducting sphere of radius $r_{0}$ is placed in a (previously) uniform electric field $E_{0}$. 

![[Pasted image 20231207185254.png]]

The electrostatic potential satisfies $\nabla^{2}V=0$, since there are no free charges. Using spherical polar coordinates this potential cna be written as 

$$
V(r,\theta) = \sum_{n=0}^\infty a_{n} r^{n} P_{n}(\cos\theta) + \sum_{n=0}^\infty b_{n} r^{-n-1}P_{n}(\cos \theta)\left( 1-\frac{r_{0}^{3}}{r^{3}} \right).
$$
Using appropriate boundary conditions, show that 

$$
V(r,\theta)=-E_{0} r P_{1}(\cos \theta) \left( 1- \frac{r_{0}^{3}}{r^{3}} \right) .
$$
This potential function can now be used for the calculation of the induced charge on the conducting sphere as a function of $\theta$ or the induced dipole moment.

***


6. Show that for associated Legendre functions:

**a)** $P_{n}^{m}(-x)=(-1)^{n+m} P_{n}^{m}(x).$
**b)** $P_{l}^{l}(x) = \frac{(2l)!}{2^{l}(l!)}(1-x^{2})^{l/2}$
**c)** $P_{l+1}^{l}(x) = x(2l+1)P_{l}^{l}$


***